fix interleave; add Wait constructor and interpretation

iocy/iocy.fst
@@ -10,7 +10,7 @@ type run 'e (a:Type u#a) =
 
 noeq
 type runtree 'e (a:Type u#a) : Type u#a =
-| Node : run 'e a -> list u#a (runtree 'e (Universe.raise_t unit)) -> runtree 'e a
+| Node : run 'e a -> list (runtree 'e (Universe.raise_t unit)) -> runtree 'e a
 
 let rec interleave (t1:trace 'e) (t2:trace 'e) : list (trace 'e) =
   match t1, t2 with
@@ -28,44 +28,93 @@ let _ =
   assert (interleave #int [1;2] [0] == [ [1;2;0]; [1;0;2]; [0;1;2] ]);
   assert (flatten (map (interleave [0]) [[]]) == [ [0] ])
 
-let rec reduce (l:list (trace 'e)) (acc:list (trace 'e)) : list (trace 'e) =
-  match l with
-  | [] -> acc
-  | h::tl -> reduce tl (flatten (map (interleave h) acc))
+let product (xs:list 'a) (ys:list 'b) : list ('a * 'b) =
+  concatMap (fun x -> map (fun y -> (x, y)) ys) xs
+
+let uncurry (f:'a -> 'b -> 'c) ((a,b):('a * 'b)) : 'c = f a b
+
+let interleave_lists (#e:Type0) l1 l2 : list (trace e) = 
+  match l1, l2 with
+  | [], [] -> []
+  | [], l2 -> l2
+  | l1, [] -> l1
+  | _, _ -> concatMap (uncurry interleave) (product l1 l2)
 
 val (===) : list 'a -> list 'a -> Type0
 let (===) l1 l2 = forall e. e `memP` l1 <==> e `memP` l2
 
 let _ =
-//  assert (reduce #int [[]; [1;2]] [[]] == [ [1;2] ]) by (compute (); dump "h");
-  assert (reduce #int [[1;2];[]] [[]] === [ [1;2] ]);
-  assert (reduce #int [[1;2]] [[0]] === [ [1;2;0]; [0;1;2]; [1;0;2] ])
-  
-let rec as_trace (t:runtree 'e 'a) : list (trace 'e) =
+  assert (interleave_lists [[]; [1;2]] [[]] == [ [1;2] ]);
+  assert (interleave_lists [[1;2];[]] [[]] === [ [1;2] ]);
+  assert (interleave_lists [[1;2]] [[0]] === [ [1;2;0]; [0;1;2]; [1;0;2] ])
+
+let _ =
+  assert (interleave_lists #int [[0;1;2];[0;2;1]] [[5;6]] === [
+      [0; 1; 2; 5; 6]; [0; 1; 5; 2; 6]; [0; 1; 5; 6; 2]; [0; 5; 1; 2; 6]; [0; 5; 1; 6; 2];
+      [0; 5; 6; 1; 2]; [5; 0; 1; 2; 6]; [5; 0; 1; 6; 2]; [5; 0; 6; 1; 2]; [5; 6; 0; 1; 2];
+      [0; 2; 1; 5; 6]; [0; 2; 5; 1; 6]; [0; 2; 5; 6; 1]; [0; 5; 2; 1; 6]; [0; 5; 2; 6; 1];
+      [0; 5; 6; 2; 1]; [5; 0; 2; 1; 6]; [5; 0; 2; 6; 1]; [5; 0; 6; 2; 1]; [5; 6; 0; 2; 1]
+    ]) by (compute ())
+
+let rec reduce (f:'a -> 'b -> 'b) (x:'b) (l:list 'a) : Tot 'b (decreases l) =
+match l with
+| [] -> x
+| h::tl -> reduce f (f h x) tl
+
+let reduce_interleave (l:list (list (trace 'e))) : list (trace 'e) = reduce (interleave_lists) [] l
+
+let _ =
+  assert (reduce_interleave ([[[2]]]) == [ [2] ]);
+  assert (reduce_interleave ([[[]];[[2]]]) == [ [2] ])
+
+let rec as_traces (t:runtree 'e 'a) : list (trace 'e) =
   match t with
   | Node (Cv _ lt) rts -> 
-    admit ();
-    map (append lt) (reduce (filter (fun l -> l <> []) (concatMap as_trace rts)) [[]])
+    admit (); (** proof of termination needed **)
+    let trs : list (list (trace 'e)) = map as_traces rts in
+    let trs : list (trace 'e) = reduce_interleave trs in
+    if List.length trs > 0 then map (append lt) trs
+    else [lt]
 
+let _ = 
+  assert (map (as_traces #unit #int) [
+             Node (Cv () [ ]) [];
+             Node (Cv () [2]) []] === [[[]];[[2]]]) by (compute ())
+
+let _ =
+  assert (
+         as_traces #unit #int (Node (Cv () [1])
+            [Node (Cv (Universe.raise_val ()) [ ]) [];
+             Node (Cv (Universe.raise_val ()) [2]) []])
+          === [ [1;2] ])
 
 let _ = 
   assert (
-         as_trace #unit #int (Node (Cv () [1])
-            [Node (Cv (Universe.raise_val ()) [ ]) [];
-             Node (Cv (Universe.raise_val ()) [2]) []])
-          == [ [1;2] ]) by (compute ());
-  assert (
-         as_trace #unit #int (Node (Cv () [1])
+         as_traces #unit #int (Node (Cv () [1])
             [Node (Cv (Universe.raise_val ()) [0]) [];
              Node (Cv (Universe.raise_val ()) [2]) []])
-          === [ [1;0;2]; [1;2;0] ]) by (compute ());
+          === [ [1;0;2]; [1;2;0] ]) by (compute ())
+
+let _ =
   assert (
-         as_trace #unit #int (Node (Cv () [])
+         as_traces #unit #int (Node (Cv () [])
             [Node (Cv (Universe.raise_val ()) [0]) [];
              Node (Cv (Universe.raise_val ()) [1]) [
                Node (Cv (Universe.raise_val ()) [ ]) [];
                Node (Cv (Universe.raise_val ()) [2]) []]])
           === [ [1;0;2]; [1;2;0]; [0;1;2] ]) by (compute ())
+
+let _ = 
+  assert (
+      as_traces #unit #int (Node (Cv () [])
+        [Node (Cv (Universe.raise_val ()) [0])
+            [Node (Cv (Universe.raise_val ()) [1]) []; Node (Cv (Universe.raise_val ()) [2]) []];
+          Node (Cv (Universe.raise_val ()) [5; 6]) []]) == [
+      [5; 6; 0; 2; 1]; [5; 0; 6; 2; 1]; [5; 0; 2; 6; 1]; [5; 0; 2; 1; 6]; [0; 5; 6; 2; 1];
+      [0; 5; 2; 6; 1]; [0; 5; 2; 1; 6]; [0; 2; 5; 6; 1]; [0; 2; 5; 1; 6]; [0; 2; 1; 5; 6];
+      [5; 6; 0; 1; 2]; [5; 0; 6; 1; 2]; [5; 0; 1; 6; 2]; [5; 0; 1; 2; 6]; [0; 5; 6; 1; 2];
+      [0; 5; 1; 6; 2]; [0; 5; 1; 2; 6]; [0; 1; 5; 6; 2]; [0; 1; 5; 2; 6]; [0; 1; 2; 5; 6]]) by (compute ())
+
 
 let rec univ_ch (t:runtree 'e (Universe.raise_t u#0 u#a unit)) : runtree 'e (Universe.raise_t u#0 u#b unit) =
 match t with
@@ -81,54 +130,57 @@ let rec prepend_rt (lt:list 'e) (rt:runtree 'e 'a) : Tot (runtree 'e 'a) (decrea
   | Node (Cv x lt') rt -> Node (Cv x (lt@lt')) (map #(runtree 'e (Universe.raise_t unit)) (prepend_rt lt) rt)
 
 type hist_post 'e 'a = runtree 'e 'a -> Type0
-type hist_pre 'e = trace 'e -> Type0
+type hist_pre 'e (a:Type u#a) = list (runtree 'e (Universe.raise_t u#0 u#a unit)) -> trace 'e -> Type0
 
-type hist0 'e 'a = hist_post 'e 'a -> hist_pre 'e
+type hist0 'e 'a = hist_post 'e 'a -> hist_pre 'e 'a
 
 let hist_post_ord (p1 p2:hist_post 'e 'a) = forall r. p1 r ==> p2 r
 
 let hist_wp_monotonic (wp:hist0 'e 'a) =
-  forall p1 p2. (p1 `hist_post_ord` p2) ==> (forall h. wp p1 h ==> wp p2 h)
+  forall p1 p2. (p1 `hist_post_ord` p2) ==> (forall ths h. wp p1 ths h ==> wp p2 ths h)
 
-type hist 'e a = wp:(hist0 'e a){hist_wp_monotonic wp}
+type hist 'e 'a = wp:(hist0 'e 'a){hist_wp_monotonic wp}
 
 let hist_return (#e:Type0) (x:'a) : hist e 'a =
-  fun p _ -> p (Node (Cv x []) [])
+  fun p _ _ -> p (Node (Cv x []) [])
 
 let hist_post_shift (p:hist_post 'e 'b) (rt:runtree 'e 'a) : hist_post 'e 'b =
   fun (rt':runtree 'e 'b) -> 
     match rt, rt' with
-      | Node (Cv x lt) trt, Node (Cv x' lt') trt' -> p (Node (Cv x' (lt@lt')) ((univ_change trt) @ trt'))
+    | Node (Cv x lt) trt, Node (Cv x' lt') trt' -> p (Node (Cv x' (lt@lt')) ((univ_change trt) @ trt'))
 
 let hist_post_bind
+  (#a:Type u#a) (#b:Type u#b)
+  (ths:list (runtree 'e (Universe.raise_t u#0 u#b unit)))
   (h:trace 'e)
-  (kw : 'a -> hist 'e 'b)
-  (p:hist_post 'e 'b) :
-  Tot (hist_post 'e 'a) =
-  fun (rt:runtree 'e 'a) ->
-    let (x,lt) = (match rt with | Node (Cv x lt) _ -> (x,lt)) in
-    kw x (hist_post_shift p rt) (List.rev lt @ h)
+  (kw : a -> hist 'e b)
+  (p:hist_post 'e b) :
+  Tot (hist_post 'e a) =
+  fun (rt:runtree 'e a) ->
+    match rt with | Node (Cv x lt) rts ->
+    kw x (hist_post_shift p rt) ((univ_change rts)@ths) (List.rev lt @ h)
 
-let hist_bind0 (w : hist 'e 'a) (kw : 'a -> hist 'e 'b) : hist0 'e 'b =
-  fun p h -> w (hist_post_bind h kw p) h
+let hist_bind0 (#a:Type u#a) (#b:Type u#b) (w : hist 'e a) (kw : a -> hist 'e b) : hist0 'e b =
+  fun p ths h -> w (hist_post_bind ths h kw p) (univ_change ths) h
 
-let hist_bind (w : hist 'e 'a) (kw : 'a -> hist 'e 'b) : hist 'e 'b =
+let hist_bind (#a:Type u#a) (#b:Type u#b) (w : hist 'e a) (kw : a -> hist 'e b) : hist 'e b =
   let wp =   hist_bind0 w kw in
   assume (hist_wp_monotonic wp);
   wp
 
 val hist_ord : hist 'e 'a -> hist 'e 'a -> Type0
-let hist_ord wp1 wp2 = forall h p. wp1 p h ==> wp2 p h
+let hist_ord wp1 wp2 = forall ths h p. wp1 p ths h ==> wp2 p ths h
 
 val hist_equiv : hist 'e 'a -> hist 'e 'a -> Type0
-let hist_equiv wp1 wp2 = forall h p. wp1 p h <==> wp2 p h
+let hist_equiv wp1 wp2 = forall h thrs p. wp1 p thrs h <==> wp2 p thrs h
 
 noeq
 type free (a:Type u#a) (e:Type0) : Type u#(max 1 a)=
+| Require : (pre:pure_pre) -> cont:((squash pre) -> free u#a a e) -> free a e
 | Return : a -> free a e
 | Print : (arg:e) -> cont:(unit -> free u#a a e) -> free a e
 | Fork : th:(unit -> free (Universe.raise_t unit) e) -> cont:(unit -> free a e) -> free a e
-| Require : (pre:pure_pre) -> cont:((squash pre) -> free u#a a e) -> free a e
+| Wait : nat -> cont:(unit -> free a e) -> free a e
 
 let free_return (#a:Type) (#e:Type) (x:a) : free a e =
   Return x
@@ -152,18 +204,20 @@ let rec free_bind
   | Require pre fnc ->
       Require pre (fun _ ->
         free_bind (fnc ()) k)
+  | Wait id fnc ->
+      Wait id (fun i -> free_bind (fnc i) k)
 
 let hist_require #e (pre:pure_pre) : hist e (squash pre) = 
-  let wp' : hist0 e (squash pre) = fun p h -> pre /\ p (Node (Cv () []) []) in
-  assert (forall post1 post2. (hist_post_ord post1 post2 ==> (forall h. wp' post1 h ==> wp' post2 h)));
+  let wp' : hist0 e (squash pre) = fun p _ _ -> pre /\ p (Node (Cv () []) []) in
+  assert (forall post1 post2. (hist_post_ord post1 post2 ==> (forall h thrs. wp' post1 thrs h ==> wp' post2 thrs h)));
   assert (hist_wp_monotonic wp');
   wp'
 
 let hist_print (#e:Type) (ev:e) : hist e unit =
-  fun p _ -> p (Node (Cv () [ev]) [])
+  fun p _ _ -> p (Node (Cv () [ev]) [])
 
 let hist_fork0 (#e:Type u#0) (#a:Type u#a) (hist_th:hist e (Universe.raise_t u#0 u#a unit)) : hist0 e (Universe.raise_t u#0 u#a unit) =
-  fun p h -> hist_th (fun r -> p (Node (Cv (Universe.raise_val ()) []) [r])) h
+  fun p -> hist_th (fun r -> p (Node (Cv (Universe.raise_val ()) []) [r]))
 
 let hist_fork (#e:Type u#0) (#a:Type u#a) (hist_th:hist e (Universe.raise_t u#0 u#a unit)) : hist e (Universe.raise_t u#0 u#a unit) =
   let wp = hist_fork0 #e #a hist_th in
@@ -173,32 +227,39 @@ let hist_fork (#e:Type u#0) (#a:Type u#a) (hist_th:hist e (Universe.raise_t u#0 
 val theta : free 'a 'e -> hist 'e 'a
 let rec theta m =
   match m with
-  | Return x -> hist_return x
   | Require pre k ->
       hist_bind (hist_require pre) (fun r -> theta (k r))
+  | Return x -> hist_return x
   | Print arg k ->
       hist_bind (hist_print arg) (fun r -> theta (k r))
   | Fork th k -> (
-    let wp = fun p h -> 
+    let wp = fun p thrs h -> 
       theta (th ()) (fun rt -> 
         theta (k ()) (fun rt' -> 
           let (Node (Cv x lt) thrs) = rt' in
           p (Node (Cv x []) [rt; (Node (Cv (Universe.raise_val ()) lt) thrs) ])
-        ) h
-      ) h in
+        ) ((univ_ch rt)::thrs) h
+      ) thrs h in
     assume (hist_wp_monotonic wp);
     wp
   )
-      //hist_bind (hist_fork #string #a (theta (th ()))) (fun _ -> theta (k ()))
+  | Wait id k -> let wp = (fun p thrds h ->
+    match List.Tot.Base.nth thrds id with
+    | None -> True 
+    | Some rt ->
+    (forall lt. lt `memP` as_traces rt ==>
+      theta (k ()) (fun (Node (Cv x lt') rts) -> p (Node (Cv x lt') rts)) thrds (** - rt **) (List.rev lt @ h))) in
+    assume (hist_wp_monotonic wp);
+    wp
 
-#reset-options
+
 let result (r:runtree 'e 'a) : 'a =
   match r with
   | Node (Cv x _) _ -> x
   
 let prog0 =  Print 0 (fun () -> Print 1 (fun () -> Print 2 (fun () -> Return 5)))
 
-let _ = assert (theta prog0 (fun r -> result r == 5 /\ as_trace r === [[0; 1; 2]]) [])  by (norm [delta_only [`%prog0; `%theta;`%hist_print;`%hist_bind;`%hist_fork;`%hist_fork0;`%hist_bind0;`%hist_post_bind;`%hist_return;`%hist_post_shift;`%univ_change;`%univ_ch];zeta;iota]; 
+let _ = assert (theta prog0 (fun r -> result r == 5 /\ as_traces r === [[0; 1; 2]]) [] [])  by (norm [delta_only [`%prog0; `%theta;`%hist_print;`%hist_bind;`%hist_fork;`%hist_fork0;`%hist_bind0;`%hist_post_bind;`%hist_return;`%hist_post_shift;`%univ_change;`%univ_ch];zeta;iota]; 
 
   l_to_r [`List.Tot.Properties.append_l_nil;`List.Tot.Properties.append_nil_l];
   compute ())
@@ -208,26 +269,33 @@ let prog1 = Fork (fun () -> Print 0 (fun () -> Return (Universe.raise_val ())))
                                                   (fun () -> Return ())))
 
 
-let _ = assert (theta prog1 (fun r -> as_trace r === [[1; 0; 2]; [1; 2; 0]; [0; 1; 2]]) [])  by (norm [delta_only [`%prog1; `%theta;`%hist_print;`%hist_bind;`%hist_fork;`%hist_fork0;`%hist_bind0;`%hist_post_bind;`%hist_return;`%hist_post_shift;`%univ_change;`%univ_ch];zeta;iota]; 
-
-  l_to_r [`List.Tot.Properties.append_l_nil;`List.Tot.Properties.append_nil_l];
-  compute ())
+let _ = assert (theta prog1 (fun r -> as_traces r === [[1; 0; 2]; [1; 2; 0]; [0; 1; 2]]) [] []) by (compute ())
 
 let prog2 =  Print 0 
                  (fun () -> Print 1 (fun () -> Fork (fun () -> Print 2 (fun () -> Return (Universe.raise_val ())))
                                                 (fun () -> Return 5)))
 
-let _ = assert (theta prog2 (fun r -> result r == 5 /\ as_trace r === [[0; 1; 2]]) [])  by (norm [delta_only [`%prog2; `%theta;`%hist_print;`%hist_bind;`%hist_fork;`%hist_fork0;`%hist_bind0;`%hist_post_bind;`%hist_return;`%hist_post_shift;`%univ_change;`%univ_ch];zeta;iota]; 
-
-  l_to_r [`List.Tot.Properties.append_l_nil;`List.Tot.Properties.append_nil_l];
-  compute ())
+let _ = assert (theta prog2 (fun r -> result r == 5 /\ as_traces r === [[0; 1; 2]]) [] [])  by (compute ())
 
 
 let prog3 = Fork (fun () -> Print 0 (fun () -> Fork (fun () -> Print 2 (fun () -> Return (Universe.raise_val ())))
                                                  (fun () -> Return (Universe.raise_val ()))))
                  (fun () -> Print 1 (fun () -> Return ()))
 
-let _ = assert (theta prog3 (fun r -> result r == () /\ as_trace r === [[0; 2; 1];[0;1;2];[1;0;2]]) [])  by (norm [delta_only [`%prog2; `%theta;`%hist_print;`%hist_bind;`%hist_fork;`%hist_fork0;`%hist_bind0;`%hist_post_bind;`%hist_return;`%hist_post_shift;`%univ_change;`%univ_ch];zeta;iota]; 
+let _ = assert (theta prog3 (fun r -> result r == () /\ as_traces r === [[0; 2; 1];[0;1;2];[1;0;2]]) [] []) by (compute ())
 
-  l_to_r [`List.Tot.Properties.append_l_nil;`List.Tot.Properties.append_nil_l];
-  compute ())
+let prog4 = Fork (fun () -> Print 0 (fun () -> Return (Universe.raise_val ()))) 
+                 (fun () -> Print 5 (fun () -> Wait 0 (fun () -> Print 6 (fun () -> Return ()))))
+
+let _ = assert (theta prog4 (fun r -> result r == () /\ as_traces r == [[0; 5; 6];[5;0;6]]) [] [])  by (  compute ();
+  dump "h";
+  tadmit ())
+
+let prog5 = Fork (fun () -> Print 0 (fun () -> Fork (fun () -> Print 1 (fun () -> Return (Universe.raise_val ())))
+                                                 (fun () -> Print 2 (fun () -> Return (Universe.raise_val ())))))
+                 (fun () -> Print 5 (fun () -> Wait 0 (fun () -> Print 6 (fun () -> Return ()))))
+
+
+let _ = assert (theta prog5 (fun r -> result r == () /\ as_traces r == [[0;1;2;5;6];[0;2;1;5;6];[0;2;5;1;6];[0;5;2;1;6];[0;5;2;1;6]]) [] [])  by (
+  compute ();
+  dump "h")
